Prove equivalence between two Hoare triples
One is the natural definition, directly in terms of execution, the other
is about arbitrary continuations and uses a Hoare double. This is a
clean statement that the reflected triples are given exactly the right
meaning.

It seems like the Hoare double definition is generally more useful
(specs chain nicely), but for any metatheory the triples are easier to
reason about.

src/OptimisticTranslator.v
@@ -45,7 +45,57 @@ Section OptimisticTranslator.
           | None => None
           end.
 
-  Theorem spec_to_exec : forall tid A T (spec: Spec A T) a p,
+  (* this is really the natural interpretation of a triple, directly as a
+  correctness statement - [cprog_triple] instead unquotes triple into a double
+  (with an arbitrary continuation) and then uses the double-based correctness
+  statement *)
+  (* TODO: this is basic metatheory, it should be elsewhere *)
+  (* TODO: [cprog_triple'] and [cprog_triple] need better names *)
+  Definition cprog_triple' A T tid (spec: Spec A T) (p: @cprog St T) :=
+    forall a st out,
+      precondition (spec a st) ->
+      exec G tid st p out ->
+      match out with
+      | Finished sigma_i' sigma' v => postcondition (spec a st) (sigma_i', sigma') v
+      | Error => False
+      end.
+
+  Theorem triple_triple'_equiv : forall A T tid (spec: Spec A T) (p: @cprog St T),
+      cprog_triple G tid spec p <->
+      cprog_triple' tid spec p.
+  Proof.
+    unfold cprog_triple, ReflectDouble, cprog_triple'.
+    split; intros.
+    - unfold cprog_ok at 1 in H.
+      specialize (H _ Ret st).
+      specialize (H (fun st' v => postcondition (spec a st) st' v)).
+      specialize (H out).
+
+      apply H.
+
+      exists a; intuition eauto.
+      unfold cprog_ok; intros.
+      CCLTactics.inv_ret; intuition (subst; eauto).
+
+      apply monad_right_id; auto.
+    - unfold cprog_ok at 1; intros; repeat deex.
+      CCLTactics.inv_bind.
+      match goal with
+      | [ Hexec: exec _ _ _ p _ |- _ ] =>
+        eapply H in Hexec; intuition eauto
+      end.
+      match goal with
+      | [ Hexec: exec _ _ _ (rx _) _ |- _ ] =>
+        eapply H2 in Hexec; intuition eauto
+      end.
+
+      match goal with
+      | [ Hexec: exec _ _ _ p _ |- _ ] =>
+        eapply H in Hexec; intuition eauto
+      end.
+  Qed.
+
+  Corollary spec_to_exec : forall tid A T (spec: Spec A T) a p,
       cprog_triple G tid spec p ->
       forall st out,
       exec G tid st p out ->
@@ -56,19 +106,11 @@ Section OptimisticTranslator.
         | Error => False
       end.
   Proof.
-    unfold cprog_triple, ReflectDouble; intros.
-    unfold cprog_ok at 1 in H.
-    specialize (H _ Ret st).
-    specialize (H (fun st' v => postcondition (spec a st) st' v)).
-    specialize (H out).
-
-    apply H.
-
-    exists a; intuition eauto.
-    unfold cprog_ok; intros.
-    CCLTactics.inv_ret; intuition (subst; eauto).
-
-    apply monad_right_id; auto.
+    intros.
+    destruct (triple_triple'_equiv tid spec p); intuition.
+    match goal with
+    | [ H: cprog_triple' _ _ _ |- _ ] => eapply H; eauto
+    end.
   Qed.
 
   Hint Resolve locally_modified_refl.
